RelationalCalculus/Applied/Sudoku/Defs.lean
@@ -1,0 +1,87 @@
+import Mathlib.Data.Finset.Basic
+import Mathlib.Tactic
+
+
+namespace Sudoku
+
+def Value : Finset Nat := {1,2,3,4,5,6,7,8,9}
+
+def v (n : Nat) (h : n ∈ Value := by first | decide ) : { x // x ∈ Value } := ⟨n, h⟩
+
+-- instance : Coe Nat  { x // x ∈ Value }  where
+--   coe n :=  toValue n
+
+def vasdasd : Value := v 1
+
+def OptionalValue := Option Value
+
+structure Place where
+  -- The 3 x 3 square numbered from upper left then left to right in three big rows
+  sector: Value
+  -- The row top to bottom
+  row: Value
+  -- The column left to right
+  col: Value
+  -- If the board position has a fixed value
+  fixedValue: Option Value
+  -- If fixed value is non-empty this must match.
+  assignedValue:  Option Value
+deriving Repr, DecidableEq
+
+def Place.empty (sector: Value)(col: Value)(row: Value) := Place.mk sector col row none none
+
+
+def one : Value := ⟨ 1, by decide ⟩
+def two : Value := ⟨ 2, by decide ⟩
+def three : Value := ⟨ 3, by decide ⟩
+set_option diagnostics true
+def sector1NoValues : List Place :=
+let empty  := Place.empty one
+[
+  empty one one, empty one two, empty one three,
+  empty two one, empty two two, empty two three,
+  empty three one, empty three two, empty three three,
+]
+
+#check (· %· : Nat -> Nat -> Nat )
+#eval 1 - (1 % 3)
+
+def getSector (row: Value) (col: Value) :=
+ let rEdge := row.val - (row.val % 3)
+ let cEdge := col.val - (col.val % 3)
+ match cEdge,rEdge with
+ | 0, 0 => 1
+ | 3, 0 => 2
+ | 6, 0 => 3
+ | 0, 3 => 4
+ | 3, 3 => 5
+ | 6, 3 => 6
+ | 0, 6 => 7
+ | 3, 6 => 8
+ | 6, 6 => 9
+ | _,_ => sorry
+
+#eval getSector 1 1
+
+
+
+def shiftCol (n: Nat)(p: Place) :=
+let raw := p.col.val + n
+match raw with
+| m + 10   => p
+| v => {p with col := ⟨raw, sorry ⟩ }
+
+
+
+
+-- def getInitialPlace (sector: Value) (col: ) (n: Value) (l: List Place ) : List Place :=
+-- match n.val with
+-- | m + 1 =>
+
+
+
+-- A valid {arg} assignment
+
+
+
+end Sudoku
