RelationalCalculus/Inclusion.lean
@@ -1,0 +1,137 @@
+
+import RelationalCalculus.Basic
+import RelationalCalculus.Order
+import RelationalCalculus.Eq
+import RelationalCalculus.Element
+import Mathlib.Tactic
+
+namespace Relation
+open Relation
+
+-- This should define the set of pairs in R which are not in S, that is it is R - S.
+def subtract {α β :Type u} (R S: Relation α β ) := (copy α)▹(R ⊗ S⁻)▹(merge β)
+infixl: 60 "⊖" => subtract -- \ominus
+
+theorem subtract_eval {α β :Type u} {R S: Relation α β} : eval (R ⊖ S) = fun (a:α ) (b:β) => (R.eval a b) ∧ (¬S.eval a b) := by
+  simp [eval, domain, codomain]
+  funext a b
+  simp
+  constructor
+  · intro h
+    rcases h with ⟨a1,a2,⟨a_a1,a_a2⟩, Ra1b, nSa2b⟩
+    constructor
+    · rwa [a_a1.symm] at Ra1b
+    · rwa [a_a2.symm] at nSa2b
+  · intro h
+    rcases h with ⟨Rab, nSab⟩
+    use a, a
+
+-- If R - S is empty then R is less than or equal to S
+theorem rel_inclusion {α β :Type u} {R S: Relation α β} : (R ⊖ S ≈ empty α β) = (R ≤ S) := by
+    simp [(·≈·), eq, (·≤·), eval, domain, codomain]
+
+-- We prove that subtracting the difference between R and S form R gives a subrelation of S
+theorem difference_subrelation {α β :Type u} (R S: Relation α β) : R⊖(R⊖S) ≤ S := by
+ simp [(·≤·), eval, domain, codomain]
+ intro a b Rab RabSab
+ exact RabSab Rab
+
+-- theorem sfdsdf  {α β :Type u} (R S: Relation α β) :∀ (a:α )(b:β), eval R-S a b →
+
+-- theorem sdfd {α β :Type u} {R S T: Relation α β} {h1: R ≤ S}{h2: T ≤ S}:
+
+theorem largest_subrelation {α β :Type u} {R S T: Relation α β} : T ≤ S → (T ≤ R⊖(R⊖S)) := by
+  have RdiffSubS: R⊖(R⊖S) ≤ S := difference_subrelation R S
+  simp [(·≤·), eval, domain, codomain]
+  simp [(·≤·), (·⊖·), merge, eval, domain, codomain] at RdiffSubS
+  intro TsubS
+  have h1 : T ⊖ R ≈ empty α β := by
+   simp [(·≈·), eq, (·≤·), eval, domain, codomain]
+   intro a b
+   by_contra nTR
+   push_neg at nTR
+   obtain ⟨Tab, nRab⟩ := nTR
+   specialize TsubS a b
+   specialize RdiffSubS a b
+   have Sab := TsubS Tab
+   -- I should be able to prove a contradition from Sab : S.eval a b, nRab : ¬R.eval a b ... actually not sure...
+
+
+
+  intro h a b Tab
+  constructor
+  · sorry
+  ·
+
+
+def relInclusion {α β :Type u} (R S: Relation α β ) := (R ⊗ S⁻)⁻
+infixl : 50 "⊑" => relInclusion
+
+def disjunctiveRelInclusion {α β :Type u} (R S: Relation α β ) := (R⁻ ⊕ S)⁻
+
+
+
+
+-- This appears not to hold if α or β are empty.
+theorem le_then_inclusion {α β :Type u}  [hα: Nonempty α] [hβ :Nonempty β] (R S: Relation α β) : R ≤ S → isNonEmpty (R ⊑ S) := by
+  simp [isNonEmpty, (·⊑·), relInclusion, (· ≤ · ), domain, codomain, eval]
+  intro h
+  by_cases hR : ∃ a b, R.eval a b
+  · rcases hR with ⟨a, b, hRab⟩
+    use a, a, b, b
+    intro _
+    exact h a b hRab
+  · simp at hR
+    let a := Classical.choice hα
+    let b := Classical.choice hβ
+    use a, a, b, b
+    intro hRab
+    exfalso
+    exact hR a b hRab
+
+
+
+theorem inclusion_then_le {α β :Type u}  [hα: Nonempty α] [hβ :Nonempty β] (R S: Relation α β) :  isNonEmpty (R ⊑ S) → R ≤ S  := by
+  simp [isNonEmpty, (·⊑·), relInclusion, (· ≤ · ), domain, codomain, eval]
+  -- Give friendly names to variables and re-order
+  intro a1 a2 b1 b2 RS a b hab
+  revert a b ; revert  a2 b2 ; revert a1  b1
+
+  have hImp :  (∀ (a1 : α) (b1 : β) (a2 : α) (b2 : β), (R.eval a1 b1 → S.eval a2 b2)) → (∃ (a3: α)(b3: β), eval R a3 b3) → S ≈ (full α β)  := by
+    intro h ex
+    rcases ex with ⟨a3,b3, Ra3b3⟩
+    specialize h a3 b3
+    have isTrue : R.eval a3 b3 = True := by aesop
+    rw [isTrue] at h
+    simp at h
+    simp [(· ≈·), eq,(· ≤ · ), eval ]
+    exact h
+
+  have hImpR :  (S ≈ (full α β)) →  (∀ (a1 : α) (b1 : β) (a2 : α) (b2 : β), (R.eval a1 b1 → S.eval a2 b2)) := by
+   simp [(· ≈·), eq,(· ≤ · ), eval ]
+   intro hSab a1 b1 a2 b2
+   specialize hSab a2 b2
+   aesop
+
+  have converseHImpR : ¬ (∀ (a1 : α) (b1 : β) (a2 : α) (b2 : β), (R.eval a1 b1 → S.eval a2 b2)) → ¬ (S ≈ (full α β)) := by aesop
+
+  by_cases RImpS : ∀ (a1 : α) (b1 : β) (a2 : α) (b2 : β), (R.eval a1 b1 → S.eval a2 b2)
+  · by_cases  Rab:  ∃ (a3: α)(b3: β), eval R a3 b3
+    · have Sfull := hImp RImpS Rab
+      aesop
+    · aesop
+  · intro a1 b1 a2 b2
+    have spec : ¬  R.eval a1 b1 → S.eval a2 b2 := by
+      sorry
+    sorry
+
+
+    -- have SNotFull := converseHImpR RImpS
+    -- push_neg at RImpS
+    -- rcases RImpS with ⟨a1,b1,a2, b2,Ra1b1, notSa2b2⟩
+
+
+  --  <;> by_cases  Rab:  ∃ (a3: α)(b3: β), eval R a3 b3
+    -- ·
+
+    -- have sddf := hImp ⟨RS, Rab⟩
