RelationalCalculus/NewToSort.lean
@@ -1,0 +1,217 @@
+import RelationalCalculus.Basic
+import RelationalCalculus.Order
+import RelationalCalculus.Eq
+import RelationalCalculus.Element
+import Mathlib.Logic.Equiv.Basic
+import Mathlib.Tactic
+
+
+-- NOTE: There is some good stuff in here but I need to organize it and figure out which is worth keeping.
+
+open Relation
+
+
+@[simp]
+lemma product_congr  {α β γ δ : Type u}{ R R': Relation α β} {S S': Relation γ δ} (hR: R ≈ R') (hS: S ≈ S') : R⊗S  ≈ R'⊗S' := by
+ simp [(· ≈ · ), eq, (· ≤ · ), eval]
+ constructor <;> intro a c b d Rab Scd
+ · constructor
+   · rwa [eq_to_eval hR.symm]
+   · rwa [eq_to_eval hS.symm]
+ · constructor
+   · rwa [eq_to_eval hR]
+   · rwa [eq_to_eval hS]
+
+@[simp]
+lemma coproduct_congr  {α β γ δ : Type u}{ R R': Relation α β} {S S': Relation γ δ} (hR: R ≈ R') (hS: S ≈ S') : (R⊕S)  ≈ (R'⊕S') := by
+ simp [(· ≈ · ), eq, (· ≤ · ), eval]
+ constructor <;>  constructor
+ · intro a b Rab
+   rwa [eq_to_eval hR.symm]
+ · intro c d Scd
+   rwa [eq_to_eval hS.symm]
+ · intro a b Rab
+   rwa [eq_to_eval hR]
+ · intro c d Scd
+   rwa [eq_to_eval hS]
+
+
+@[simp]
+lemma comp_congr_left {α β γ : Type u}{ R R': Relation α β} {S: Relation β  γ } (hR: R ≈ R') : (R▹S)  ≈ (R'▹S)  := by
+ simp [(· ≈ · ), eq, (· ≤ · ), eval, domain]
+ constructor <;> intro a c b Rab Sbc <;> use b
+ · rw [eq_to_eval hR.symm]
+   exact ⟨Rab, Sbc⟩
+ · rw [eq_to_eval hR.symm] at Rab
+   exact ⟨Rab, Sbc⟩
+
+@[simp]
+lemma comp_congr_right {α β γ : Type u}{ R: Relation α β} {S S': Relation β  γ } (hS: S ≈ S') : (R▹S)  ≈ (R▹S')  := by
+ simp [(· ≈ · ), eq, (· ≤ · ), eval, domain]
+ constructor <;> intro a c b Rab Sbc <;> use b
+ · rw [eq_to_eval hS.symm]
+   exact ⟨Rab, Sbc⟩
+ · rw [eq_to_eval hS.symm] at Sbc
+   exact ⟨Rab, Sbc⟩
+
+def coprodFromProd {α β γ δ : Type u} (R: Relation (α × γ) (β × δ)) : Relation (Sum α  γ) (Sum β δ) :=  (first α γᵒ▹R▹first β δ) ⊕ ((second α γᵒ)▹R▹second β δ)
+
+def prodFromCoprod {α β γ δ : Type u} (R: Relation (Sum α  γ) (Sum β δ)) :  Relation (α × γ) (β × δ) :=  (left α γ▹R▹left β δᵒ) ⊗ (right α γ▹R▹right β δᵒ)
+
+
+-- We can only recover R if S is non-empty since otherwise, we have no elemetns in R⊗S.
+theorem recover_first_of_prod  {α β γ δ : Type u} (R: Relation α β) (S: Relation γ δ) (hNE: isNonEmpty S) :  R ≈ (first α γᵒ ▹ (R⊗S) ▹ first β δ) := by
+simp  [(· ≈ · ), eq, (· ≤ · ),  eval]
+simp [isNonEmpty,(· ≤ · ), eval] at hNE
+
+
+have hLeft : ∀ (a : α) (b : β), R.eval a b → R.eval a b ∧ ∃ x x_1, S.eval x_1 x := by
+  intro a b Rab
+  constructor
+  · assumption
+  · obtain ⟨c, h⟩ := hNE
+    obtain ⟨d, h⟩ := h
+    use d ; use c
+
+have hRight : (∀ (a : α) (b : β), R.eval a b → ∀ (x : δ) (x_1 : γ), S.eval x_1 x → R.eval a b) := by
+  intro a b Rab d c _ ; assumption
+
+exact ⟨ hLeft, hRight ⟩
+
+
+
+-- We can only recover S if R is non-empty since otherwise, we have no elemetns in R⊗S.
+theorem recover_second_of_prod  {α β γ δ : Type u} (R: Relation α β) (S: Relation γ δ) (hNE: isNonEmpty R) :  S ≈ (second α γᵒ ▹ (R⊗S) ▹ second β δ)  := by
+simp  [(· ≈ · ), eq, (· ≤ · ),  eval]
+simp [isNonEmpty,(· ≤ · ), eval] at hNE
+intro a b Sab;
+obtain ⟨a', h⟩ := hNE
+obtain ⟨b', h⟩ := h
+constructor
+· use b' ; use a'
+· exact Sab
+
+
+theorem recover_left_of_coprod  {α β γ δ : Type u} (R: Relation α β) (S: Relation γ δ) : R ≈  (left α γ ▹ R⊕S ▹ left β δᵒ)  := by
+simp  [(· ≈ · ), eq, (· ≤ · ), prodFromCoprod, eval]
+
+theorem recover_right_of_coprod  {α β γ δ : Type u} (R: Relation α β ) (S: Relation γ δ ) : S ≈ (right α γ ▹ R⊕S ▹ right β δᵒ) := by simp  [(· ≈ · ), eq, (· ≤ · ), prodFromCoprod, eval]
+
+
+theorem coproduct_equiv_prod  {α β γ δ : Type u} (R: Relation α β ) (S: Relation γ δ )  : (prodFromCoprod (R⊕S)) ≈ (R⊗S) := by
+  simp [prodFromCoprod]
+  have h1 :=  recover_left_of_coprod R S
+  have h2 :=  recover_right_of_coprod R S
+  have h3 := product_congr h1 h2
+  exact h3.symm
+
+-- I might not need this
+theorem atom_prod_coprod  {α β γ δ : Type u} {R: Relation (α × γ) (β × δ)} : eval (coprodFromProd R) =  (fun(v1: Sum α γ) => fun ( v2: Sum β δ ) =>
+    match v1, v2 with
+    | Sum.inl a, Sum.inl b => ∃ c' d', eval R (a, c') (b, d')
+    | Sum.inr c, Sum.inr d => ∃ a' b', eval R (a', c) (b', d)
+    | _,_ => False
+)  := by
+simp [coprodFromProd, eval]
+ext x x_1 : 3
+cases x with
+| inl val =>
+  cases x_1 with
+  | inl val_1 =>
+    simp_all only
+    constructor <;>
+    intro a <;> obtain ⟨d, c, h⟩ := a <;> use c <;> use d
+  | inr val_2 => simp_all only
+| inr val_1 =>
+  cases x_1 with
+  | inl val => simp_all only
+  | inr val_2 =>
+    simp_all only
+    constructor <;> intro a
+    <;>  obtain ⟨b, a, h⟩ := a
+    <;>  use a <;> use b
+
+-- I might not need this
+theorem atom_coprod_prod  {α β γ δ : Type u} {R: Relation (Sum α γ) (Sum β δ)} : eval (prodFromCoprod R) =  (fun ((a,c):  α × γ) ((b,d): β × δ) =>
+  (eval R (Sum.inl a) (Sum.inl b)) ∧ eval R (Sum.inr c) (Sum.inr d)) := by
+  simp  [(· ≈ · ), eq, (· ≤ · ), prodFromCoprod, eval]
+
+
+
+
+-- coprodFromProd will have R inl a inl b and R inr c inr d iff R has (a, b)(c,d)
+
+theorem prod_imp_coprod_conjunction {α β γ δ : Type u} {R: Relation α β } {S: Relation γ δ }  : ∀ (a: α )(c : γ) (b : β ) (d: δ), ((R⊗S).eval (a,c) (b,d)) → (((coprodFromProd (R⊗S)).eval (Sum.inl a) (Sum.inl b)) ∧ ((coprodFromProd (R⊗S)).eval (Sum.inr c) (Sum.inr d)))  := by
+ intro a c b d
+ rw [atom_prod_coprod]
+ simp [eval]
+ intro Rab Scd
+ constructor
+ · constructor
+   ·  exact Rab
+   · use c ; use d
+ · constructor
+   · use a ; use b
+   · exact Scd
+
+theorem  coprod_conjunction_imp_prod {α β γ δ : Type u} {R: Relation α β } {S: Relation γ δ }  : ∀ (a: α )(c : γ) (b : β ) (d: δ),  (((coprodFromProd (R⊗S)).eval (Sum.inl a) (Sum.inl b)) ∧ ((coprodFromProd (R⊗S)).eval (Sum.inr c) (Sum.inr d))) → ((R⊗S).eval (a,c) (b,d)) := by
+ intro a c b d
+ rw [atom_prod_coprod]
+ simp [eval]
+ intro Rab c' d' _ a' b' _ Scd
+ constructor <;> assumption
+
+
+theorem prod_eq_coprod_conjunction  {α β γ δ : Type u} {R: Relation α β } {S: Relation γ δ }  : ∀ (a: α )(c : γ) (b : β ) (d: δ), ((R⊗S).eval (a,c) (b,d)) = (((coprodFromProd (R⊗S)).eval (Sum.inl a) (Sum.inl b)) ∧ ((coprodFromProd (R⊗S)).eval (Sum.inr c) (Sum.inr d)))  := by
+ intro a b c d
+ simp
+ constructor
+ · exact prod_imp_coprod_conjunction a b c d
+ · exact  coprod_conjunction_imp_prod a b c d
+
+
+-- A product can be converted to a coproduct and back again.
+theorem product_inverse  {α β γ δ : Type u} {R: Relation α β } {S: Relation γ δ }  : R⊗S  ≈ prodFromCoprod (coprodFromProd (R⊗S))   := by
+simp only [(· ≈ · ), eq, (· ≤ · )]
+rw [atom_coprod_prod, atom_prod_coprod]
+simp_all
+constructor
+· intro a c b d RS
+  constructor
+  · use c ; use d
+  · use a ; use b
+·   intro a c b d c' d'
+    -- TODO: Modify prod_eq_coprod_conjunction so it works without applying explicit arguments. Maybe I need to make a c b d implicit arguments as well.
+    have h := @prod_eq_coprod_conjunction α β γ δ R S a c' b d'
+    rw [h ]
+    simp [eval]
+    intro Rab d3 c3 _ b3 a3 _ _ a4 b4 _ Scd
+    constructor <;> assumption
+
+
+
+-- Interesting. So I discovered that you can't recover the coproduct when one of the sides is empty.
+theorem coproduct_inverse  {α β γ δ : Type u} {R: Relation α β } {S: Relation γ δ }   (hNER: isNonEmpty R)(hNES: isNonEmpty S): (R⊕S)  ≈ coprodFromProd (prodFromCoprod (R⊕S))   := by
+  have h : prodFromCoprod (R ⊕ S) ≈ R ⊗ S := coproduct_equiv_prod R S
+  have hFirst : (first α γᵒ ▹ prodFromCoprod (R ⊕ S) ▹ first β δ) ≈ (first α γᵒ ▹ R⊗S ▹ first β δ) := by
+    have h4 : (first α γᵒ ▹ prodFromCoprod (R ⊕ S)) ≈ (first α γᵒ ▹ R⊗S) := by exact comp_congr_right h
+    exact comp_congr_left h4
+
+  have hSecond : (second α γᵒ ▹ prodFromCoprod (R ⊕ S) ▹ second β δ) ≈ (second α γᵒ ▹ R⊗S ▹ second β δ) := by
+    have h4 : (second α γᵒ ▹ prodFromCoprod (R ⊕ S)) ≈ (second α γᵒ ▹ R⊗S) := by exact comp_congr_right h
+    exact comp_congr_left h4
+  simp only [coprodFromProd]
+  have hEquiv := coproduct_congr hFirst hSecond
+  apply symm
+  apply (instSetoid.iseqv.trans hEquiv)
+
+
+  have hCoprod : (R ⊕ S) ≈ (first α γᵒ ▹ R ⊗ S ▹ first β δ) ⊕ (second α γᵒ ▹ R ⊗ S ▹ second β δ) := by
+    have hLeft : R ≈ (first α γᵒ ▹ R ⊗ S ▹ first β δ) := by
+      exact recover_first_of_prod R S hNES
+    have hRight : S ≈ (second α γᵒ ▹ R ⊗ S ▹ second β δ) := by
+      exact recover_second_of_prod R S hNER
+    exact coproduct_congr hLeft hRight
+  apply (instSetoid.iseqv.trans hCoprod.symm)
+  simp_all
+  rfl
